03_PROTO/target/debug/deps/teras_lang_types-f165529ab72657a0.d
@@ -1,5 +1,0 @@
-/workspaces/proof/03_PROTO/target/debug/deps/teras_lang_types-f165529ab72657a0.d: crates/teras-lang-types/src/lib.rs
-
-/workspaces/proof/03_PROTO/target/debug/deps/libteras_lang_types-f165529ab72657a0.rmeta: crates/teras-lang-types/src/lib.rs
-
-crates/teras-lang-types/src/lib.rs:
