03_PROTO/target/debug/deps/terasc-a0d1985d0caff20e.d
@@ -1,5 +1,0 @@
-/workspaces/proof/03_PROTO/target/debug/deps/terasc-a0d1985d0caff20e.d: crates/terasc/src/main.rs
-
-/workspaces/proof/03_PROTO/target/debug/deps/terasc-a0d1985d0caff20e: crates/terasc/src/main.rs
-
-crates/terasc/src/main.rs:
